only verification error is compare expecting bool and not CompResult.

src/CompariosRelations.dfy
@@ -4,8 +4,8 @@ module Relations.ComparisonsRelation {
 
     export 
     reveals Reflexive, AntiSymmetric, Connected, TotalOrdering
-
     import opened Helpers.Comparison
+
 
     predicate Reflexive<T(!new)>(R: (T, T) -> CompResult) 
     {
@@ -26,7 +26,19 @@ module Relations.ComparisonsRelation {
     {
     && Reflexive(R)
     && AntiSymmetric(R)
-    && Helpers.Transitive(R)
+    && Transitive(R)
     && Connected(R)
     }  
+
+        predicate Trichotomous<T(!new)>(less: (T, T) -> CompResult) 
+    {
+        (forall x, y :: less(x, y) || x == y || less(y, x)) &&  // at least one of the three
+        (forall x, y :: less(x, y) && less(y, x) ==> false) &&  // not both of the less's
+        (forall x, y :: less(x, y) ==> x != y)  // not a less and the equality
+    }
+
+    predicate Transitive<T(!new)>(R: (T, T) -> CompResult) 
+    {
+        forall x, y, z :: R(x, y) && R(y, z) ==> R(x, z)
+    }
 }
